New notation for pure judgements

coq-osiris/theories/program_logic/pure/pure_notation.v
@@ -2,25 +2,30 @@ From osiris Require Import base.
 From osiris.lang Require Import lang.
 From osiris.semantics Require Import code eval.
 
+From osiris.program_logic.pure Require Import pure_judgement.
+
 (** Notational typeclasses for pure hoare triples. *)
 
 (* Value predicates, which are predicates over carrier type [A], which are *)
 (*    encodable types. *)
-Structure vPred :=
-  { vpred : forall {A} `{Encode A}, (A → Prop) -> val -> Prop }.
+Definition returns {A} `{Encode A} (φ : A -> Prop):=
+  λ v, ∃ a, v = #a ∧ φ a.
 
-Canonical Structure vPred_Instance : vPred :=
-  {| vpred := λ _ _  φ v, ∃ a, v = #a ∧ φ a |}.
+(* Class of judgements over [micro] expressions, which are lifted over encodable
+  values. *)
+Class Judgement :=
+  jm : forall {A E} `{Encode A}, micro val E -> (A -> Prop)-> Prop.
 
-Class Pure := pure : forall {A E}, micro A E -> vPred -> Prop.
+(* The default instantiation of a judgement uses the pure predicate. *)
+#[global] Instance PureJudgement : Judgement :=
+  fun _ _ _ a Φ => pure a (returns Φ) ⊥.
 
-Notation "'EXPR' e 'REQUIRES' Φ" :=
-  (pure e Φ)
-   (at level 20, e, Φ at level 200,
-     format "'[hv' 'EXPR'  e '/' 'REQUIRES'  Φ ']'").
+Notation "'{' η ⊢ e 'ensures' Φ '}'" :=
+  (jm (eval η e) Φ)
+   (at level 80, e, Φ at level 100,
+     format "'[hv' '{'  η  '⊢'  '/' e  '/' 'ensures'  Φ  '}' ']'").
 
-Notation "'ENV' η 'EXPR' e 'REQUIRES' Φ" :=
-  (pure (eval η e) Φ)
-   (at level 20, e, Φ at level 200,
-     format "'[hv' 'ENV'  η '/' 'EXPR'  e '/' 'REQUIRES' Φ ']'").
-
+Notation "'{' e 'ensures' Φ '}' " :=
+  (jm e Φ)
+   (at level 80, e, Φ at level 200,
+     format "'[hv' '{'  e  '/' 'ensures'  Φ  '}' ']'").
