coq-osiris/theories/program_logic/program_logic.v
@@ -1,5 +1,8 @@
 (* This file summarizes the content of program_logic/ directory. *)
 
+From osiris.program_logic.pure Require Export
+     pure.
+
 From osiris.program_logic Require Export
      ewp
      basic_rules
